ISLPrograms.fst
@@ -2,23 +2,51 @@ module ISLPrograms
 
 open IncSepLogic
 
+(*
+n := 1000000;
+i, j := 0;
+while (i <= n){
+  i++;
+  if (random()) j++;
+}
+assert  (j != n);
+*)
+
+let ( ||| ) = Choice
+
+let enot (e : expr) : expr = Minus (Const 1) e
+let ge (x y : expr) : expr = enot (Lt x y)
+
 // n := 1000000; i := 0; j := 0;
 unfold let init_vars = 
-  Seq (Assign "n" (Const 1000000))
-      (Seq (Assign "i" (Const 0)) (Assign "j" (Const 0)))
+  Assign "n" (Const 1000000) `Seq`
+  Assign "i" (Const 0) `Seq`
+  Assign "j" (Const 0)
 
 // el cuerpo del while
 let loop_body =
-  Seq (Assume (Lt (Var "i") (Var "n")))
-      (Seq (Assign "i" (Plus (Var "i") (Const 1)))
-           (Choice Skip (Assign "j" (Plus (Var "j") (Const 1)))))
+  Assume (Lt (Var "i") (Var "n")) `Seq`
+  Assign "i" (Plus (Var "i") (Const 1)) `Seq`
+  (Assign "j" (Plus (Var "j") (Const 1)) ||| Skip)
 
 let assert_stmt =
-  Choice (Seq (Assume (Eq (Var "j") (Var "n"))) Error)
-         (Choice (Seq (Assume (Lt (Var "j") (Var "n"))) Skip)
-                 (Seq (Assume (Gt (Var "j") (Var "n"))) Skip))
+  Seq (Assume (Eq (Var "j") (Var "n"))) Error |||
+  Assume (enot (Eq (Var "j") (Var "n")))
 
 unfold let prog1 =
-  Seq init_vars
-      (Seq (Kleene loop_body)
-           (Seq (Assume (Eq (Var "i") (Var "n"))) assert_stmt))
+  init_vars `Seq`
+  Kleene loop_body `Seq`
+  Assume (ge (Var "i") (Var "n")) `Seq`
+  assert_stmt
+
+
+(*
+  {true}
+  x = alloc()
+  *x = 1
+  {er: x=NULL}
+*)
+(*
+  x = alloc()
+  free(x)
+*)
